# 第7章 递推关系和生成函数

## EX1

> Let $f_0, f_1, f_2, ..., f_n, ...$, denote the Fibonacci sequence. By evaluating each of the following expressions for small values of n, conjecture a general formula and then prove it, using mathematical induction and the Fibonacci recurrence:
>
> (a) $f_1 + f_3 + \cdots + f_{2n-1}$
>
> (b) $f_0 + f_2 + \cdots + f_{2n}$
>
> (c) $f_0 - f_1 + f_2 - \cdots + (-1)^n f_n$
>
> (d)$f_0^2 + f_1^2 + \cdots + f_n^2$

### EX1(a)

先打表找规律，

```cpp
#include <iostream>
#include <vector>

using namespace std;

int main()
{
    int p = 0, q = 1;
    vector<int> fibList {p, q};
    for(int i = 0; i < 50; ++ i) {
        fibList.emplace_back(p+q);
        p = q;
        q = fibList.back();
    }
    
    int odd_total = 0, even_total = 0, alter_total = 0, square_total;
    int flag = 1;
    printf("idx \t sum_odd \t sum_total \t sum_alter \t sum_square \n");
    for(int i = 0; i < 10; ++ i) {
        odd_total += fibList[max(2*i-1, 0)];
        even_total += fibList[2*i];
        alter_total += flag * fibList[i];
        flag *= -1;
        square_total += fibList[i] * fibList[i];
        printf("%d \t %d \t %d \t %d \t %d\n", i, odd_total, even_total,
                alter_total, square_total);
    }
    return 0;
}
```

可以发现：$f_1 + f_3 + \cdots + f_{2n-1} = f_{2n}$，$f_0 + f_2 + \cdots + f_{2n} = f_{2n-1}-1$，$f_0 - f_1 + f_2 - \cdots + (-1)^n f_n = -1 + (-1)^n f_{n-1}$，$f_0^2 + f_1^2 + \cdots + f_n^2 = f_n f_{n+1}$。

数学归纳证明过程略。

### EX1(d)

这个强调一下特殊的构造方法，辅助猜测递推公式。

$$
\begin{aligned}
    \sum_{i = 0}^{n} f_i &= f_0^2 + \sum_{i=1}^n f_i^2 \\
    &= f_0 f_1 + \sum_{i=1}^n f_i (f_{i+1} - f_{i-1}) \\
    &= f_0 f_1 + (f_1f_2 - f_1f_0) + (f_2 f_3 - f_2 f_1) + \cdots + (f_nf_{n+1} - f_n f_{n-1}) \\
    &= f_n f_{n+1}
\end{aligned}
$$

## EX2

> Prove that the nth Fibonacci number In is the integer that is closest to the number
> $$
> \frac{1}{\sqrt{5}} {\left( \frac{1+\sqrt{5}}{2} \right)^n}
> $$

设$a = \frac{1}{\sqrt{5}} {\left( \frac{1+\sqrt{5}}{2} \right)^n}$，并且知道$f_n = \frac{1}{\sqrt{5}} {\left( \frac{1+\sqrt{5}}{2} \right)^n} - \frac{1}{\sqrt{5}} {\left( \frac{1-\sqrt{5}}{2} \right)^n}$，那么$f_n$与a的距离为，

$$
\begin{aligned}
    |f_n - a| = & \left|\frac{1}{\sqrt{5}} {\left( \frac{1-\sqrt{5}}{2} \right)}^n \right| \\
    =& \frac{1}{\sqrt{5}} {\left( \frac{(\sqrt{5}-1)(\sqrt{5}+1)}{2(\sqrt{5}+1)} \right)}^n \\
    =& \frac{1}{\sqrt{5}} \left(\frac{2}{\sqrt{5}+1}\right)^n \\
    \le &\frac{1}{\sqrt{5}} \frac{2}{\sqrt{5}+1} \\
    = & \frac{2}{5 + \sqrt{5}} \\
    \le & \frac{2}{5}
\end{aligned}
$$

因此，$f_n$是最接近$\frac{1}{\sqrt{5}} {\left( \frac{1+\sqrt{5}}{2} \right)^n}$的整数。

## EX3

> Prove the following about the Fibonacci numbers:
>
> (a) $f_n$ is even if and only if n is divisible by 3.
>
> (b) $f_n$ is divisible by 3 if and only if n is divisible by 4.
>
> (c) $f_n$ is divisible by 4 if and only if n is divisible by 6.

### EX3(b)

$f_0 = 0,f_1 = f_2 = 1, f_3 = 2, f_4 = 3, \cdots$，$f_0$能被3整除，且n=0可被4整除。并且$f_1, f_2, f_3$均不能被3整除，$f_4=3$可被3整除，且n=4被4整除。

下面使用数学归纳法证明，当n被4整除时，$f_n$一定被3整除。

设$f_{4m}$被3整除，且$m \ge 1$。

$$
\begin{aligned}
    f_{4m+4} =& f_{4m+3} + f_{4m+2} \\
    =& 2f_{4m+2} + f(4m+1) \\
    =& 3f_{4m+1} + f_{4m}
\end{aligned}
$$

f_{4m+4}被3整除。

### EX3PS

暂时有些问题，没有准确论证「必要性」。或许可以从「周期性」的角度入手。

## EX4

> Prove that the Fibonacci sequence is the solution of the recurrence relation
> $$
> a_n = 5a_{n-4} + 3 a_{n-5}, \quad (n \ge 5),
> $$
> where ao = 0, al = 1, a2 = 1, a3 = 2, and U4 = 3. Then use this formula to show that the Fibonacci numbers satisfy the condition that $f_n$ is divisible by 5 if and only if n is divisible by 5.

连续使用$a_n = a_{n-1} + a_{n-2}$进行代换，

$$
\begin{aligned}
    a_n =& a_{n-1} + a_{n-2} \\
    =& 2a_{n-2} + a_{n-3} \\
    =& 3a_{n-3} + 2a_{n-4} \\
    =& 5a_{n-4} + 3a_{n-5}
\end{aligned}
$$

因此$a_n$与$a_{n-5}$模5同余，即$a_n \equiv a_{n-5} (mod~5)$。并且由$a_0=0,a_1 = 1, a_2=1, a_3=2,a_4=3$可知，当且仅当n被5整除时，$f_{n}~mod~5=0$。

## EX5

> By examining the Fibonacci sequence, make a conjecture about when $f_n$ is divisible by 7 and then prove your conjecture.

对斐波那契数列$f_n$能被7整除，当且仅当n能被8整除。

## EX6-7

越来越懒了，**加星题**，题目都不想抄了。

## EX8

> Consider a 1-by-n chessboard. Suppose we color each square of the chessboard with one of the two colors red and blue. Let hn be the number of colorings in which no two squares that are colored red are adjacent. Find and verify a recurrence relation that hn satisfies. Then derive a formula for hn .

如果第一个方块着成红色，那么第二个方块只能着成蓝色，问题转化为$1\times (n-2)$棋盘着色问题；如果第一个方块着成蓝色，问题转化为$1\times (n-1)$期盼着色问题；因此，$h_n = h_{n-1} + h_{n-2}$。

并且有初始项$h_0 = 1, h_1 = 2$，显然$h_n = f_{n+2}$。

## EX9

> Let $h_n$ equal the number of different ways in which the squares of a 1-by-n chessboard can be colored, using the colors red, white, and blue so that no two squares that are colored red are adjacent. Find and verify a recurrence relation that $h_n$ satisfies. Then find a formula for $h_n$.

考虑第一个方框放红色，那么第二个方块只能放白色或蓝色，问题转化为$h_{n-2}$；考虑第一个方块放白色或蓝色，那么问题转化为$h_{n-1}$。

$$
h_{n} = 2h_{n-1} + 2h_{n-2}, \quad h_0 = 1, h_1 = 3
$$

求解方程$x^2 = 2x+2$，对应$h_n$的通解为$h_n = c_1 (1+\sqrt{3})^n + c_2 (1-\sqrt{3})^n$。

带入初始值$h_0 = 1, h_1 = 3$可以求出常系数$c_1 = \frac{1}{2} + \frac{\sqrt{3}}{3}, c_2 = \frac{1}{2} - \frac{\sqrt{3}}{3}$。

$$
h_n = \frac{3+2\sqrt{3}}{6} (1+\sqrt{3})^n + \frac{3-2\sqrt{3}}{6}(1-\sqrt{3})^n, \quad n =0, 1, 2, \cdots
$$

## EX10

> Suppose that, in his problem, Fibonacci had placed two pairs of rabbits in the enclosure at the beginning of a year. Find the number of pairs of rabbits in the enclosure after one year. More generally, find the number of pairs of rabbits in the enclosure after n months.

设第n个月时有$g_n$个兔子，满足$g_n = g_{n-1} + g_{n-2}, g_0 = 0, g_1 = 2$，可以求出通解，

$$
g_n = \frac{2}{\sqrt{5}} \left( \frac{1+\sqrt{5}}{2} \right)^n - \frac{2}{\sqrt{5}} \left( \frac{1-\sqrt{5}}{2} \right)^n = 2f_n
$$

第n个月的数量为$g_n$个，第一个月后的n个月是第n+1月，因此有$g_{n+1}$对兔子。

### EX10注

本身有些文字游戏的味道，如果要问「一共有多少**只**兔子？」是不是也能算作一道题目呢。

## EX11

> The Lucas numbers $l_0, l_1, l_2, \cdots, l_n, \cdots$ are defined using the same recurrence relation defining the Fibonacci numbers, but with different initial conditions:
> $$
> l_n = l_{n-1} + l_{n-2}, \quad (n \ge 2), l_0 =2, l_1 = 1
> $$
> Prove that
>
> (a) $l_n = f_{n-1} + f_{n+1} \text{ for } n \ge 1$
>
> (b) $l_0^2 + l_1^2 + \cdots + l_n^2  = l_n l_{n+1} + 2 \text{ for } n \ge 0$

### EX11(a)

设$Z_n = f_{n-1} + f_{n+1} - l_{n}, n \ge 1$，$Z_1 = f_0 + f_2 - l_1 = 0 + 1 - 1 = 0$；$Z_2 = f_1 + f_3 - l_2 = 1 + 2 - 3 = 0$。

又因为$Z_n = Z_{n-1} + Z_{n-2}, n \ge 3$，所以$Z_n = 0, n \ge 1$。即有，

$$
l_n = f_{n-1} + f_{n+1}, \quad n \ge 1
$$

### EX11(b)

因为$l_{n+1} = l_n + l_{n-1}$，所以$l_n^2 = l_n (l_{n+1} - l_{n-1}), n \ge 1$。

$$
\begin{aligned}
    l_0^2 + l_1^2 + \cdots + l_n^2 =& l_0^2 + \sum_{i=1}^{n} l_i^2 \\
    =& 4 + (l_1l_2 - l_1l_0) + (l_2l_3 - l_2l_1) + \cdots + (l_{n}l_{n+1} - l_nl_{n-1}) \\
    =& 4 + l_n l_{n+1} - l_1l_0 \\
    =& l_n l_{n+1} + 2
\end{aligned}
$$

## EX12

> Let $h_0, h_1, h_2, \cdots, h_n, \cdots$ be the sequence defined by
>$$
>h_n = n^3, \quad (n \ge 0)
>$$
>Show that $h_n = h_{n-1} + 3n^2 -3n + 1$ is the recurrence relation for the sequence.

带入$h_{n-1} = (n-1)^3$化简。

## EX13

> Determine the generating function for each of the following sequences:
> (a) c^0 =1, c, c^2, ..., c^n, ...
>
> (b) $1, -1, 1, -1, ..., (-1)^n$, ...
>
> (c) $\dbinom{\alpha}{0}, -\dbinom{\alpha}{1}, \dbinom{\alpha}{2}, ... , (-1)^n \dbinom{\alpha}{n}, ... ,$ ($\alpha$ is a real number)
>
> (d) $1, \frac{1}{1!}, \frac{1}{2!}, ..., \frac{1}{n!}, ...$
>
> (e) $1, -\frac{1}{1!}, \frac{1}{2!}, ..., (-1)^n \frac{1}{n!}, ...$

无穷数列$h_0, h_1, h_2, \cdots, h_n， \cdots$对应的生成函数为

$$
g(x) = h_0 + h_1x + h_2 x^2 + \cdots + h_n x^n \cdots
$$

### EX13(a)

$$
\begin{aligned}
    g(x) =& 1 + cx + c^2 x^2 + \cdots + c^n x^n  + \cdots \\
    =& 1 + (cx) + (cx)^2 + \cdots + (cx)^n + \cdots \\
    =&\frac{1}{1-cx}
\end{aligned}
$$

### EX13(b)

$$
\begin{aligned}
    g(x) =& 1 - x + x^2 + \cdots + (-1)^n x^n  + \cdots \\
    =& 1 + (-x) + (-x)^2 + \cdots + (-x)^n + \cdots \\
    =&\frac{1}{1+x}
\end{aligned}
$$

### EX13(c)

$$
\begin{aligned}
    g(x) =& \binom{\alpha}{0} - \binom{\alpha}{1} x + \binom{\alpha}{2} x^2 + \cdots + (-1)^n \binom{\alpha}{n} x^n  + \cdots \\
    =& \sum_{k=0}^{\infty} \binom{\alpha}{k} (-x)^k \\
    =& (1-x)^\alpha
\end{aligned}
$$

### EX13(d)

$$
\begin{aligned}
    g(x) =& 1 + \frac{1}{1!} x + \frac{1}{2!} x^2 + \cdots + \frac{1}{n!} x^n  + \cdots \\
    = &e^x
\end{aligned}
$$

### EX13(e)

$$
\begin{aligned}
    g(x) =& 1 - \frac{1}{1!} x + \frac{1}{2!} x^2 - \cdots + (-1)^n \frac{1}{n!} x^n  + \cdots \\
    =& e^{-x}
\end{aligned}
$$

## EX14

> Let S be the multiset $\{\infty \cdot e_1, \infty \cdot e_2, \infty \cdot e_3, \infty \cdot e_4\}$ Determine the generating function for the sequence $h_0, h_1, h_2, \cdots, h_n， \cdots$, where $h_n$ is the number of n-combinations of S with the following added restrictions:
> (a) Each $e_i$ occurs an odd number of times.
>
> (b) Each $e_i$ occurs a multiple-of-3 number of times.
>
> (c) The element $e_1$ does not occur, and $e_2$ occurs at most once.
>
> (d) The element $e_1$ occurs 1,3, or 11 times, and the element $e_2$ occurs 2,4, or 5 times.
>
> (e) Each $e_i$ occurs at least 10 times.

### EX14(a)

$$
\begin{aligned}
    g(x) =&( x +  x^3 + x^5 + \cdots )( x +  x^3 + x^5 + \cdots )( x +  x^3 + x^5 + \cdots )( x +  x^3 + x^5 + \cdots ) \\
    = & \left( \frac{x}{1-x^2} \right)^4
\end{aligned}
$$

### EX14(b)

$$
\begin{aligned}
    g(x) =&( 1 +  x^3 + x^6 + \cdots )( 1 +  x^3 + x^6 + \cdots )( 1 +  x^3 + x^6 + \cdots )( 1 +  x^3 + x^6 + \cdots ) \\
    = & \frac{1}{(1-x^3)^4}
\end{aligned}
$$

### EX14(c)

$$
\begin{aligned}
    g(x) =&( 1 )(1 + x)(1 + x + x^2 + x^3 + \cdots )(1 + x + x^2 + x^3 + \cdots ) \\
    = & \frac{1+x}{(1-x)^2}
\end{aligned}
$$

### EX14(d)

$$
\begin{aligned}
    g(x) =&( x+x^3+x^{11})(x^2 + x^4 + x^5)(1 + x + x^2 + x^3 + \cdots )(1 + x + x^2 + x^3 + \cdots ) \\
    = & \frac{(x+x^3+x^{11})(x^2+x^4+x^5)}{(1-x)^2}
\end{aligned}
$$

### EX14(e)

$$
\begin{aligned}
    g(x) =&(x^{10} + x^{11} + \cdots )(x^{10} + x^{11} + \cdots )(x^{10} + x^{11} + \cdots )(x^{10} + x^{11} + \cdots ) \\
    =& x^{40}(1+x^2 + x^3 + \cdots)(1+x^2 + x^3 + \cdots)(1+x^2 + x^3 + \cdots)(1+x^2 + x^3 + \cdots) \\
    =& \frac{x^{40}}{(1-x)^4}
\end{aligned}
$$

## EX15

> Determine the generating function for the sequence of cubes
> $$
> 0, 1, 8, \cdots, n^3, \cdots
> $$

由第5章EX20知，

$$
n^3 = 6 \binom{n}{3} + 6 \binom{n}{2} + \binom{n}{1}
$$

$$
\begin{aligned}
    g(x) = & x + 8 x^ + \cdots + n^3 x^2 + \cdots \\
    =& \sum_{n=0}^{\infty} n^3 x^k \\
    =& \sum_{n=0}^{\infty}6 \binom{n}{3}x^n + \sum_{n=0}^{\infty}6\binom{n}{2}x^n + \sum_{n=0}^{\infty} \binom{n}{1}x^n \\
    =& 6x^3 \sum_{n=3}^{\infty} \binom{n}{3}x^{n-3} + 6x^2\sum_{n=2}^{\infty}\binom{n}{2}x^{n-2} + x\sum_{n=1}^{\infty} \binom{n}{1}x^{n-1} \\
    =& 6x^3 \sum_{n=0}^{\infty} \binom{n+3}{3}x^{n} + 6x^2\sum_{n=0}^{\infty}\binom{n+2}{2}x^{n} + x\sum_{n=0}^{\infty} \binom{n+1}{1}x^{n} 
\end{aligned}
$$

由第5章EX43知，

$$
\frac{1}{(1-z)^m} = \sum_{n=0}^{\infty} \binom{m+n-1}{n}z^n, \quad |z| \lt 1
$$

因此，

$$
\begin{aligned}
    g(x) =& 6x^3 \sum_{n=0}^{\infty} \binom{n+3}{3}x^{n} + 6x^2\sum_{n=0}^{\infty}\binom{n+2}{2}x^{n} + x\sum_{n=0}^{\infty} \binom{n+1}{1}x^{n} \\
    =& 6x^3 \frac{1}{(1-x)^4} + 6x^2 \frac{1}{(1-x)^3} + x \frac{1}{(1-x)^2} \\
    =& \frac{x(x^2+4x+1)}{(1-x)^4}
\end{aligned}
$$

## EX16

>Formulate a combinatorial problem for which the generating function is 
> $$
> (1+x+x^2)(1+x^2+x^4+x^6)(1+x^2+x^4+\cdots)(x+x^2+x^3+\cdots)
> $$